abs1_comb_thm/ref_rel_holds_call_lblScript.sml
@@ -1,5 +1,5 @@
-open HolKernel bossLib boolLib Parse;
-open SPI_stateTheory driver_stateTheory driver_relationTheory driver_callTheory ds_abs1_stateTheory ds_abs1_relTheory ds_abs1_initTheory ds_abs1_txTheory ds_abs1_rxTheory ds_abs1_xferTheory ref_relTheory;
+open HolKernel bossLib boolLib Parse wordsLib;
+open SPI_stateTheory SPI_relationTheory SPI_tauTheory SPI_update_regsTheory SPI_return_regsTheory driver_stateTheory driver_relationTheory driver_callTheory driver_writeTheory driver_readTheory driver_checkTheory ds_abs1_stateTheory ds_abs1_relTheory ds_abs1_initTheory ds_abs1_txTheory ds_abs1_rxTheory ds_abs1_xferTheory ref_relTheory weak_bisimulationTheory board_memTheory;
 
 val _ = new_theory "ref_rel_holds_call_lbl";
 
@@ -39,6 +39,7 @@ Cases_on `spi.state` >> rw [] >>
 (dr.state <> dr_rx_issue_disable) /\
 (dr.state <> dr_rx_read_conf) /\
 (dr.state <> dr_rx_reset_conf) /\
+(dr.state <> dr_rx_sendback) /\
 (dr.state <> dr_xfer_idle) /\
 (dr.state <> dr_xfer_fetch_conf) /\
 (dr.state <> dr_xfer_conf_issued) /\
@@ -51,7 +52,8 @@ Cases_on `spi.state` >> rw [] >>
 (dr.state <> dr_xfer_fetch_dataI) /\
 (dr.state <> dr_xfer_issue_disable) /\
 (dr.state <> dr_xfer_read_conf) /\
-(dr.state <> dr_xfer_reset_conf)` by rw [] >>
+(dr.state <> dr_xfer_reset_conf) /\
+(dr.state <> dr_xfer_sendback)` by rw [] >>
 Cases_on `ds_abs1.state` >> rw []);
 
 (* If dr.state = dr_ready, then abs1.state = abs1_ready according to ref_rel *)
@@ -89,6 +91,112 @@ Cases_on `spi.state` >> rw [] >>
 (dr.state <> dr_rx_issue_disable) /\
 (dr.state <> dr_rx_read_conf) /\
 (dr.state <> dr_rx_reset_conf) /\
+(dr.state <> dr_rx_sendback) /\
+(dr.state <> dr_xfer_idle) /\
+(dr.state <> dr_xfer_fetch_conf) /\
+(dr.state <> dr_xfer_conf_issued) /\
+(dr.state <> dr_xfer_read_txs) /\
+(dr.state <> dr_xfer_check_txs) /\
+(dr.state <> dr_xfer_write_dataO) /\
+(dr.state <> dr_xfer_read_rxs) /\
+(dr.state <> dr_xfer_check_rxs) /\
+(dr.state <> dr_xfer_read_rx0) /\
+(dr.state <> dr_xfer_fetch_dataI) /\
+(dr.state <> dr_xfer_issue_disable) /\
+(dr.state <> dr_xfer_read_conf) /\
+(dr.state <> dr_xfer_reset_conf) /\
+(dr.state <> dr_xfer_sendback)` by rw [] >>
+Cases_on `ds_abs1.state` >> rw []);
+
+(* If dr.state = dr_rx_sendback, then abs1.state = abs1_rx_reset according to ref_rel *)
+val dr_rx_sendback_imply_abs1_rx_reset = store_thm("dr_rx_sendback_imply_abs1_rx_reset",
+``!(spi:spi_state) (dr:driver_state) (ds_abs1:ds_abs1_state).
+(ref_rel ds_abs1 (dr,spi)) /\ (dr.state = dr_rx_sendback) ==>
+ds_abs1.state = abs1_rx_reset``,
+rw [] >>
+`IS_STATE_REL ds_abs1 dr spi` by fs [ref_rel_def] >>
+fs [IS_STATE_REL_def] >>
+Cases_on `spi.state` >> rw [] >>
+`(dr.state <> dr_init_pre) /\
+(dr.state <> dr_init_idle) /\
+(dr.state <> dr_init_read_req) /\
+(dr.state <> dr_init_check_rep) /\
+(dr.state <> dr_init_setting) /\
+(dr.state <> dr_ready) /\
+(dr.state <> dr_tx_idle) /\
+(dr.state <> dr_tx_fetch_conf) /\
+(dr.state <> dr_tx_conf_issued) /\
+(dr.state <> dr_tx_read_txs) /\
+(dr.state <> dr_tx_check_txs) /\
+(dr.state <> dr_tx_write_data) /\
+(dr.state <> dr_tx_read_eot) /\
+(dr.state <> dr_tx_check_eot) /\
+(dr.state <> dr_tx_issue_disable) /\
+(dr.state <> dr_tx_read_conf) /\
+(dr.state <> dr_tx_reset_conf) /\
+(dr.state <> dr_rx_idle) /\
+(dr.state <> dr_rx_fetch_conf) /\
+(dr.state <> dr_rx_conf_issued) /\
+(dr.state <> dr_rx_read_rxs) /\
+(dr.state <> dr_rx_check_rxs) /\
+(dr.state <> dr_rx_read_rx0) /\
+(dr.state <> dr_rx_fetch_data) /\
+(dr.state <> dr_rx_issue_disable) /\
+(dr.state <> dr_rx_read_conf) /\
+(dr.state <> dr_rx_reset_conf) /\
+(dr.state <> dr_xfer_idle) /\
+(dr.state <> dr_xfer_fetch_conf) /\
+(dr.state <> dr_xfer_conf_issued) /\
+(dr.state <> dr_xfer_read_txs) /\
+(dr.state <> dr_xfer_check_txs) /\
+(dr.state <> dr_xfer_write_dataO) /\
+(dr.state <> dr_xfer_read_rxs) /\
+(dr.state <> dr_xfer_check_rxs) /\
+(dr.state <> dr_xfer_read_rx0) /\
+(dr.state <> dr_xfer_fetch_dataI) /\
+(dr.state <> dr_xfer_issue_disable) /\
+(dr.state <> dr_xfer_read_conf) /\
+(dr.state <> dr_xfer_reset_conf) /\
+(dr.state <> dr_xfer_sendback)` by rw [] >>
+Cases_on `ds_abs1.state` >> rw []);
+
+(* If dr.state = dr_xfer_sendback, then abs1.state = abs1_xfer_reset according to ref_rel *)
+val dr_xfer_sendback_imply_abs1_xfer_reset = store_thm("dr_xfer_sendback_imply_abs1_xfer_reset",
+``!(spi:spi_state) (dr:driver_state) (ds_abs1:ds_abs1_state).
+(ref_rel ds_abs1 (dr,spi)) /\ (dr.state = dr_xfer_sendback) ==>
+ds_abs1.state = abs1_xfer_reset``,
+rw [] >>
+`IS_STATE_REL ds_abs1 dr spi` by fs [ref_rel_def] >>
+fs [IS_STATE_REL_def] >>
+Cases_on `spi.state` >> rw [] >>
+`(dr.state <> dr_init_pre) /\
+(dr.state <> dr_init_idle) /\
+(dr.state <> dr_init_read_req) /\
+(dr.state <> dr_init_check_rep) /\
+(dr.state <> dr_init_setting) /\
+(dr.state <> dr_ready) /\
+(dr.state <> dr_tx_idle) /\
+(dr.state <> dr_tx_fetch_conf) /\
+(dr.state <> dr_tx_conf_issued) /\
+(dr.state <> dr_tx_read_txs) /\
+(dr.state <> dr_tx_check_txs) /\
+(dr.state <> dr_tx_write_data) /\
+(dr.state <> dr_tx_read_eot) /\
+(dr.state <> dr_tx_check_eot) /\
+(dr.state <> dr_tx_issue_disable) /\
+(dr.state <> dr_tx_read_conf) /\
+(dr.state <> dr_tx_reset_conf) /\
+(dr.state <> dr_rx_idle) /\
+(dr.state <> dr_rx_fetch_conf) /\
+(dr.state <> dr_rx_conf_issued) /\
+(dr.state <> dr_rx_read_rxs) /\
+(dr.state <> dr_rx_check_rxs) /\
+(dr.state <> dr_rx_read_rx0) /\
+(dr.state <> dr_rx_fetch_data) /\
+(dr.state <> dr_rx_issue_disable) /\
+(dr.state <> dr_rx_read_conf) /\
+(dr.state <> dr_rx_reset_conf) /\
+(dr.state <> dr_rx_sendback) /\
 (dr.state <> dr_xfer_idle) /\
 (dr.state <> dr_xfer_fetch_conf) /\
 (dr.state <> dr_xfer_conf_issued) /\
@@ -132,12 +240,10 @@ val abs1_comb_hold_ref_rel_call_init = store_thm("abs1_comb_hold_ref_rel_call_in
 rw [ds_abs1_tr_cases, local_tr_cases, driver_tr_cases] >|
 [FULL_SIMP_TAC std_ss [ref_rel_def, IS_STATE_REL_def],
 rw [call_init_ds_abs1_def, call_init_dr_def] >>
-FULL_SIMP_TAC std_ss [ref_rel_def, IS_STATE_REL_def] >>
-rw [],
+FULL_SIMP_TAC std_ss [ref_rel_def, IS_STATE_REL_def] >> rw [],
 FULL_SIMP_TAC std_ss [ref_rel_def, IS_STATE_REL_def],
 rw [call_init_ds_abs1_def, call_init_dr_def] >>
-FULL_SIMP_TAC std_ss [ref_rel_def, IS_STATE_REL_def] >>
-rw []]);
+FULL_SIMP_TAC std_ss [ref_rel_def, IS_STATE_REL_def] >> rw []]);
 
 (* ds_abs1' exists for call_tx label *)
 val comb_abs1_hold_ref_rel_call_tx = store_thm("comb_abs1_hold_ref_rel_call_tx",
@@ -214,4 +320,244 @@ rw [ds_abs1_tr_cases, local_tr_cases, driver_tr_cases] >|
 rw [call_xfer_ds_abs1_def, call_xfer_dr_def] >>
 FULL_SIMP_TAC std_ss [ref_rel_def, IS_STATE_REL_def] >> rw []]);
 
+(* bisimulation: ds_abs1' exists for call_back label *)
+val comb_abs1_hold_ref_rel_call_back = store_thm("comb_abs1_hold_ref_rel_call_back",
+``!(spi:spi_state) (dr:driver_state) (ds_abs1:ds_abs1_state) (buffer:word8 list) (dr':driver_state) (ds_abs1':ds_abs1_state).
+(ref_rel ds_abs1 (dr, spi)) /\ (driver_tr dr (call_back buffer) dr') ==>
+?ds_abs1'. (ds_abs1_tr ds_abs1 (call_back buffer) ds_abs1') /\ 
+(ref_rel ds_abs1' (dr', spi))``,
+rw [driver_tr_cases,call_back_dr_data_def,call_back_dr_state_def,call_back_dr_def] >-
+(`ds_abs1.state = abs1_rx_reset` by METIS_TAC [dr_rx_sendback_imply_abs1_rx_reset] >>
+ rw [ds_abs1_tr_cases,call_back_ds_abs1_data_def,call_back_ds_abs1_state_def,
+ call_back_ds_abs1_def] >>
+ fs [ref_rel_def,IS_STATE_REL_def] >>
+ Cases_on `dr.state` >> rw []) >>
+`ds_abs1.state = abs1_xfer_reset` by METIS_TAC [dr_xfer_sendback_imply_abs1_xfer_reset] >>
+rw [ds_abs1_tr_cases,call_back_ds_abs1_data_def,call_back_ds_abs1_state_def,
+call_back_ds_abs1_def] >>
+fs [ref_rel_def,IS_STATE_REL_def] >>
+Cases_on `dr.state` >> rw []);
+
+(* bisimulation: (dr',spi') exists for call_back label *)
+val abs1_comb_hold_ref_rel_call_back = store_thm("abs1_comb_hold_ref_rel_call_back",
+``!(spi:spi_state) (dr:driver_state) (ds_abs1:ds_abs1_state) (buffer:word8 list) (ds_abs1':ds_abs1_state).
+(ref_rel ds_abs1 (dr, spi)) /\ (ds_abs1_tr ds_abs1 (call_back buffer) ds_abs1') ==>
+(?dr' spi'. (local_tr (dr, spi) (call_back buffer) (dr',spi')) /\
+(ref_rel ds_abs1' (dr', spi'))) \/
+(?n dr' spi'. (n_tau_tr n local_tr (dr,spi) (call_back buffer) (dr',spi')) /\ 
+(ref_rel ds_abs1' (dr',spi')))``,
+rw [ds_abs1_tr_cases,call_back_ds_abs1_data_def,call_back_ds_abs1_state_def,
+call_back_ds_abs1_def] >>
+`IS_STATE_REL ds_abs1 dr spi` by fs [ref_rel_def] >-
+(`(dr.state = dr_rx_sendback /\ spi.state = spi_ready) \/
+  (dr.state = dr_rx_reset_conf /\ spi.state = rx_channel_disabled) \/
+  (dr.state = dr_rx_read_conf /\ spi.state = rx_channel_disabled) \/
+  (dr.state = dr_rx_issue_disable /\ spi.state = rx_data_ready)` by fs [IS_STATE_REL_def] >|[
+  (* dr_rx_sendback and spi_ready*)
+  DISJ1_TAC >>
+  rw [local_tr_cases,driver_tr_cases,call_back_dr_state_def,call_back_dr_data_def,
+  call_back_dr_def]  >>
+  fs [ref_rel_def,IS_STATE_REL_def],
+  (* dr_rx_reset_conf and rx_channel_disabled *)
+  DISJ2_TAC >>
+  Q.EXISTS_TAC `SUC 0:num` >> 
+  fs [n_tau_tr_def,local_tr_cases, driver_tr_cases, spi_tr_cases,DR_TAU_ENABLE_def, 
+  SPI_TAU_ENABLE_def, DR_WR_ENABLE_def, DR_RD_ENABLE_def, dr_write_state_def, 
+  dr_write_value_def,dr_write_address_def, dr_write_def, dr_write_ch0conf_rx_def] >>
+  `dr.dr_last_read_v = SOME (build_CH0CONF spi.regs.CH0CONF)` by fs [ref_rel_def] >>
+  `~ (ch0conf_changed ((4293918719w:word32) && (build_CH0CONF spi.regs.CH0CONF)) spi)`
+    by (fs [build_CH0CONF_def,ch0conf_changed_def] >>
+        FULL_SIMP_TAC (std_ss++WORD_ss++WORD_BIT_EQ_ss) []) >>
+  `spi.regs.CH0CONF.FORCE = 1w` by fs [ref_rel_def] >>
+  `(20 >< 20) ((4293918719w:word32) && (build_CH0CONF spi.regs.CH0CONF)) :word1 <> spi.regs.CH0CONF.FORCE`
+  by FULL_SIMP_TAC (std_ss++WORD_ss++WORD_BIT_EQ_ss) [] >>
+  `(13 >< 12) ((4293918719w:word32) && (build_CH0CONF spi.regs.CH0CONF)): word2 = spi.regs.CH0CONF.TRM`
+  by (fs [build_CH0CONF_def] >> FULL_SIMP_TAC (std_ss++WORD_ss++WORD_BIT_EQ_ss) []) >>
+  rw [write_SPI_regs_def, SPI0_CH0CONF_def, SPI0_PA_RANGE_def,
+  SPI0_START_def, SPI0_END_def, SPI0_SYSCONFIG_def, SPI0_MODULCTRL_def,
+  write_CH0CONF_comb_def, write_CH0CONF_rx_def] >>
+  FULL_SIMP_TAC (std_ss++WORD_ss++WORD_BIT_EQ_ss) [] >>
+  rw [local_tr_cases,driver_tr_cases,call_back_dr_state_def,call_back_dr_data_def,
+  call_back_dr_def]  >>
+  fs [ref_rel_def,IS_STATE_REL_def],
+  (* dr_rx_read_conf and rx_channel_disabled *)
+  DISJ2_TAC >>
+  Q.EXISTS_TAC `SUC 1:num` >>
+  rw [n_tau_tr_def, n_tau_tr_SUC, local_tr_cases, driver_tr_cases, spi_tr_cases, DR_TAU_ENABLE_def,
+  SPI_TAU_ENABLE_def, DR_WR_ENABLE_def, DR_RD_ENABLE_def] >> 
+  `dr_read dr = dr with <|state := dr_rx_reset_conf;
+   dr_last_read_ad := SOME SPI0_CH0CONF |>` by rw [dr_read_def,dr_read_ch0conf_def] >> fs [] >>
+  `(read_SPI_regs_value SPI0_CH0CONF spi = build_CH0CONF spi.regs.CH0CONF) /\
+   (read_SPI_regs_state SPI0_CH0CONF spi = spi)`
+  by fs [read_SPI_regs_value_def,read_SPI_regs_state_def,read_SPI_regs_def,
+  SPI0_CH0CTRL_def, SPI0_PA_RANGE_def, SPI0_END_def, SPI0_START_def,SPI0_SYSSTATUS_def,
+  SPI0_SYSCONFIG_def, SPI0_MODULCTRL_def, SPI0_CH0CONF_def] >> 
+  fs [dr_write_state_def,dr_write_address_def,dr_write_value_def,
+  dr_write_def, dr_write_ch0conf_rx_def] >>
+  `~ (ch0conf_changed ((4293918719w:word32) && (build_CH0CONF spi.regs.CH0CONF)) spi)`    
+  by (fs [build_CH0CONF_def,ch0conf_changed_def] >>       
+  FULL_SIMP_TAC (std_ss++WORD_ss++WORD_BIT_EQ_ss) []) >>
+  `spi.regs.CH0CONF.FORCE = 1w` by fs [ref_rel_def] >>
+  `(20 >< 20) ((4293918719w:word32) && (build_CH0CONF spi.regs.CH0CONF)) : word1 <> 
+  spi.regs.CH0CONF.FORCE` by FULL_SIMP_TAC (std_ss++WORD_ss++WORD_BIT_EQ_ss) [] >>
+  `(13 >< 12) ((4293918719w:word32) && (build_CH0CONF spi.regs.CH0CONF)): word2 = 
+   spi.regs.CH0CONF.TRM` by (fs [build_CH0CONF_def] >>
+  FULL_SIMP_TAC (std_ss++WORD_ss++WORD_BIT_EQ_ss) []) >>
+  rw [write_SPI_regs_def, write_CH0CONF_comb_def, write_CH0CONF_rx_def, 
+  SPI0_CH0CTRL_def, SPI0_PA_RANGE_def, SPI0_END_def, SPI0_START_def,
+  SPI0_SYSCONFIG_def, SPI0_MODULCTRL_def, SPI0_CH0CONF_def] >>
+  FULL_SIMP_TAC (std_ss++WORD_ss++WORD_BIT_EQ_ss) [] >>
+  rw [local_tr_cases,driver_tr_cases,call_back_dr_state_def,call_back_dr_data_def,
+  call_back_dr_def]  >>
+  fs [ref_rel_def,IS_STATE_REL_def],
+  (* dr_rx_issue_disable and rx_data_ready *)                              
+  DISJ2_TAC >>                                  
+  Q.EXISTS_TAC `SUC 2:num` >>
+  rw [n_tau_tr_def, n_tau_tr_SUC, local_tr_cases, driver_tr_cases, spi_tr_cases, DR_TAU_ENABLE_def,
+      SPI_TAU_ENABLE_def, DR_WR_ENABLE_def, DR_RD_ENABLE_def] >>
+  `(dr_write_state dr = dr with state := dr_rx_read_conf) /\
+  (dr_write_address dr = SOME SPI0_CH0CTRL) /\
+  (dr_write_value dr = SOME (0w:word32))`
+  by rw [dr_write_state_def,dr_write_address_def,dr_write_value_def,dr_write_def,
+  dr_write_ch0ctrl_def] >> fs [] >>
+  `write_SPI_regs SPI0_CH0CTRL 0w spi =
+  spi with <|regs := spi.regs with CH0CTRL := 0w;
+             state := rx_channel_disabled|>`
+  by rw [write_SPI_regs_def, SPI0_CH0CONF_def, SPI0_PA_RANGE_def, SPI0_START_def, SPI0_END_def, 
+  SPI0_SYSCONFIG_def, SPI0_MODULCTRL_def, SPI0_CH0CTRL_def, write_CH0CTRL_def] >> fs [] >>
+  `dr_read (dr with state := dr_rx_read_conf) = dr with <|state := dr_rx_reset_conf; 
+  dr_last_read_ad := SOME SPI0_CH0CONF |>` by rw [dr_read_def,dr_read_ch0conf_def] >> fs [] >> 
+  `(read_SPI_regs_value SPI0_CH0CONF (spi with <|state := rx_channel_disabled;
+  regs := spi.regs with CH0CTRL := 0w |>) = build_CH0CONF spi.regs.CH0CONF) /\
+  (read_SPI_regs_state SPI0_CH0CONF (spi with <|state := rx_channel_disabled;
+  regs := spi.regs with CH0CTRL := 0w |>) = (spi with <|state := rx_channel_disabled;
+  regs := spi.regs with CH0CTRL := 0w |>))`
+  by fs [read_SPI_regs_value_def,read_SPI_regs_state_def,read_SPI_regs_def,
+  SPI0_CH0CTRL_def, SPI0_PA_RANGE_def, SPI0_END_def, SPI0_START_def,SPI0_SYSSTATUS_def,
+  SPI0_SYSCONFIG_def, SPI0_MODULCTRL_def, SPI0_CH0CONF_def] >> fs [] >>
+  rw [dr_write_state_def,dr_write_address_def,dr_write_value_def,
+  dr_write_def, dr_write_ch0conf_rx_def] >>
+  `~ (ch0conf_changed ((4293918719w:word32) && (build_CH0CONF spi.regs.CH0CONF)) 
+  (spi with <|state := rx_channel_disabled;
+  regs := spi.regs with CH0CTRL := 0w|>))` 
+  by (fs [build_CH0CONF_def,ch0conf_changed_def] >>
+  FULL_SIMP_TAC (std_ss++WORD_ss++WORD_BIT_EQ_ss) []) >>
+  `spi.regs.CH0CONF.FORCE = 1w` by fs [ref_rel_def] >>
+  `(20 >< 20) ((4293918719w:word32) && (build_CH0CONF spi.regs.CH0CONF)) : word1 <> 
+  spi.regs.CH0CONF.FORCE` by FULL_SIMP_TAC (std_ss++WORD_ss++WORD_BIT_EQ_ss) [] >>
+  `(13 >< 12) ((4293918719w:word32) && (build_CH0CONF spi.regs.CH0CONF)): word2 = 
+  spi.regs.CH0CONF.TRM` by (fs [build_CH0CONF_def] >>
+  FULL_SIMP_TAC (std_ss++WORD_ss++WORD_BIT_EQ_ss) []) >>
+  rw [write_SPI_regs_def, write_CH0CONF_comb_def, write_CH0CONF_rx_def, 
+  SPI0_CH0CTRL_def, SPI0_PA_RANGE_def, SPI0_END_def, SPI0_START_def,
+  SPI0_SYSCONFIG_def, SPI0_MODULCTRL_def, SPI0_CH0CONF_def] >>
+  FULL_SIMP_TAC (std_ss++WORD_ss++WORD_BIT_EQ_ss) [] >>
+  rw [local_tr_cases,driver_tr_cases,call_back_dr_state_def,call_back_dr_data_def,
+  call_back_dr_def]  >>
+  fs [ref_rel_def,IS_STATE_REL_def]]) >>
+`(dr.state = dr_xfer_sendback /\ spi.state = spi_ready) \/
+(dr.state = dr_xfer_reset_conf /\ spi.state = xfer_channel_disabled) \/
+(dr.state = dr_xfer_read_conf /\ spi.state = xfer_channel_disabled) \/
+(dr.state = dr_xfer_issue_disable /\ spi.state = xfer_ready_for_trans)` by fs [IS_STATE_REL_def] >|[
+(* dr_xfer_sendback and spi_ready *)
+DISJ1_TAC >>
+rw [local_tr_cases,driver_tr_cases,call_back_dr_state_def,call_back_dr_data_def,
+call_back_dr_def]  >>
+fs [ref_rel_def,IS_STATE_REL_def],
+(* dr_xfer_reset and xfer_channel_disabled *)
+DISJ2_TAC >>
+Q.EXISTS_TAC `SUC 0:num` >> 
+fs [n_tau_tr_def,local_tr_cases, driver_tr_cases, spi_tr_cases,DR_TAU_ENABLE_def, 
+SPI_TAU_ENABLE_def, DR_WR_ENABLE_def, DR_RD_ENABLE_def, dr_write_state_def,
+dr_write_value_def,dr_write_address_def, dr_write_def, dr_write_ch0conf_xfer_def] >>
+`dr.dr_last_read_v = SOME (build_CH0CONF spi.regs.CH0CONF)` by fs [ref_rel_def] >>
+`~ (ch0conf_changed ((4293918719w:word32) && (build_CH0CONF spi.regs.CH0CONF)) spi)` 
+by (fs [build_CH0CONF_def,ch0conf_changed_def] >>
+FULL_SIMP_TAC (std_ss++WORD_ss++WORD_BIT_EQ_ss) []) >>
+`spi.regs.CH0CONF.FORCE = 1w` by fs [ref_rel_def] >>
+`(20 >< 20) ((4293918719w:word32) && (build_CH0CONF spi.regs.CH0CONF)) :word1 <> spi.regs.CH0CONF.FORCE` by FULL_SIMP_TAC (std_ss++WORD_ss++WORD_BIT_EQ_ss) [] >>
+`(13 >< 12) ((4293918719w:word32) && (build_CH0CONF spi.regs.CH0CONF)): word2 = spi.regs.CH0CONF.TRM` by (fs [build_CH0CONF_def] >> FULL_SIMP_TAC (std_ss++WORD_ss++WORD_BIT_EQ_ss) []) >>
+rw [write_SPI_regs_def, SPI0_CH0CONF_def, SPI0_PA_RANGE_def,
+SPI0_START_def, SPI0_END_def, SPI0_SYSCONFIG_def, SPI0_MODULCTRL_def,
+write_CH0CONF_comb_def, write_CH0CONF_xfer_def] >>
+FULL_SIMP_TAC (std_ss++WORD_ss++WORD_BIT_EQ_ss) [] >>
+rw [local_tr_cases,driver_tr_cases,call_back_dr_state_def,call_back_dr_data_def,
+call_back_dr_def]  >>
+fs [ref_rel_def,IS_STATE_REL_def],   
+(* dr_xfer_read_conf and xfer_channel_disabled *)
+DISJ2_TAC >>
+Q.EXISTS_TAC `SUC 1:num` >>
+rw [n_tau_tr_def,n_tau_tr_SUC,local_tr_cases, driver_tr_cases, spi_tr_cases, DR_TAU_ENABLE_def, 
+SPI_TAU_ENABLE_def, DR_WR_ENABLE_def, DR_RD_ENABLE_def] >>
+`dr_read dr = dr with <|state := dr_xfer_reset_conf; 
+dr_last_read_ad := SOME SPI0_CH0CONF |>` by rw [dr_read_def,dr_read_ch0conf_def] >> fs [] >>
+`(read_SPI_regs_value SPI0_CH0CONF spi = build_CH0CONF spi.regs.CH0CONF) /\
+(read_SPI_regs_state SPI0_CH0CONF spi = spi)`
+by fs [read_SPI_regs_value_def,read_SPI_regs_state_def,read_SPI_regs_def,
+SPI0_CH0CTRL_def, SPI0_PA_RANGE_def, SPI0_END_def, SPI0_START_def,SPI0_SYSSTATUS_def,
+SPI0_SYSCONFIG_def, SPI0_MODULCTRL_def, SPI0_CH0CONF_def] >> 
+fs [dr_write_state_def,dr_write_address_def,dr_write_value_def,
+dr_write_def, dr_write_ch0conf_xfer_def] >>
+`~ (ch0conf_changed ((4293918719w:word32) && (build_CH0CONF spi.regs.CH0CONF)) spi)` 
+by (fs [build_CH0CONF_def,ch0conf_changed_def] >>
+FULL_SIMP_TAC (std_ss++WORD_ss++WORD_BIT_EQ_ss) []) >>
+`spi.regs.CH0CONF.FORCE = 1w` by fs [ref_rel_def] >>
+`(20 >< 20) ((4293918719w:word32) && (build_CH0CONF spi.regs.CH0CONF)) : word1 <> 
+spi.regs.CH0CONF.FORCE` by FULL_SIMP_TAC (std_ss++WORD_ss++WORD_BIT_EQ_ss) [] >>
+`(13 >< 12) ((4293918719w:word32) && (build_CH0CONF spi.regs.CH0CONF)): word2 = 
+spi.regs.CH0CONF.TRM` by (fs [build_CH0CONF_def] >>
+FULL_SIMP_TAC (std_ss++WORD_ss++WORD_BIT_EQ_ss) []) >>
+rw [write_SPI_regs_def, write_CH0CONF_comb_def, write_CH0CONF_xfer_def, 
+SPI0_CH0CTRL_def, SPI0_PA_RANGE_def, SPI0_END_def, SPI0_START_def,
+SPI0_SYSCONFIG_def, SPI0_MODULCTRL_def, SPI0_CH0CONF_def] >>
+FULL_SIMP_TAC (std_ss++WORD_ss++WORD_BIT_EQ_ss) [] >>
+rw [local_tr_cases,driver_tr_cases,call_back_dr_state_def,call_back_dr_data_def,
+call_back_dr_def]  >>
+fs [ref_rel_def,IS_STATE_REL_def],
+(* dr_xfer_issue_disable and xfer_ready_for_trans *)
+DISJ2_TAC >>
+Q.EXISTS_TAC `SUC 2:num` >>
+rw [n_tau_tr_def, n_tau_tr_SUC, local_tr_cases, driver_tr_cases, spi_tr_cases, DR_TAU_ENABLE_def, 
+SPI_TAU_ENABLE_def, DR_WR_ENABLE_def, DR_RD_ENABLE_def] >>
+`(dr_write_state dr = dr with state := dr_xfer_read_conf) /\
+(dr_write_address dr = SOME SPI0_CH0CTRL) /\
+(dr_write_value dr = SOME (0w:word32))` 
+by rw [dr_write_state_def,dr_write_address_def,dr_write_value_def,dr_write_def, 
+dr_write_ch0ctrl_def] >> fs [] >>
+`write_SPI_regs SPI0_CH0CTRL 0w spi = 
+spi with <|regs := spi.regs with CH0CTRL := 0w;
+state := xfer_channel_disabled|>` 
+by rw [write_SPI_regs_def, SPI0_CH0CONF_def, SPI0_PA_RANGE_def, SPI0_START_def, SPI0_END_def, 
+SPI0_SYSCONFIG_def, SPI0_MODULCTRL_def, SPI0_CH0CTRL_def, write_CH0CTRL_def] >> fs [] >>
+`dr_read (dr with state := dr_xfer_read_conf) = dr with <|state := dr_xfer_reset_conf; 
+dr_last_read_ad := SOME SPI0_CH0CONF |>` by rw [dr_read_def,dr_read_ch0conf_def] >> fs [] >>
+`(read_SPI_regs_value SPI0_CH0CONF (spi with <|state := xfer_channel_disabled;
+regs := spi.regs with CH0CTRL := 0w |>) = build_CH0CONF spi.regs.CH0CONF) /\
+(read_SPI_regs_state SPI0_CH0CONF (spi with <|state := xfer_channel_disabled;
+regs := spi.regs with CH0CTRL := 0w |>) = (spi with <|state := xfer_channel_disabled;
+regs := spi.regs with CH0CTRL := 0w |>))`
+by fs [read_SPI_regs_value_def,read_SPI_regs_state_def,read_SPI_regs_def,
+SPI0_CH0CTRL_def, SPI0_PA_RANGE_def, SPI0_END_def, SPI0_START_def,SPI0_SYSSTATUS_def,
+SPI0_SYSCONFIG_def, SPI0_MODULCTRL_def, SPI0_CH0CONF_def] >> fs [] >>
+rw [dr_write_state_def,dr_write_address_def,dr_write_value_def,
+dr_write_def, dr_write_ch0conf_xfer_def] >>
+`~ (ch0conf_changed ((4293918719w:word32) && (build_CH0CONF spi.regs.CH0CONF)) 
+(spi with <|state := xfer_channel_disabled;
+regs := spi.regs with CH0CTRL := 0w|>))` 
+by (fs [build_CH0CONF_def,ch0conf_changed_def] >>
+FULL_SIMP_TAC (std_ss++WORD_ss++WORD_BIT_EQ_ss) []) >>
+`spi.regs.CH0CONF.FORCE = 1w` by fs [ref_rel_def] >>
+`(20 >< 20) ((4293918719w:word32) && (build_CH0CONF spi.regs.CH0CONF)) : word1 <> 
+spi.regs.CH0CONF.FORCE` by FULL_SIMP_TAC (std_ss++WORD_ss++WORD_BIT_EQ_ss) [] >>
+`(13 >< 12) ((4293918719w:word32) && (build_CH0CONF spi.regs.CH0CONF)): word2 = 
+spi.regs.CH0CONF.TRM` by (fs [build_CH0CONF_def] >>
+FULL_SIMP_TAC (std_ss++WORD_ss++WORD_BIT_EQ_ss) []) >>
+rw [write_SPI_regs_def, write_CH0CONF_comb_def, write_CH0CONF_xfer_def, 
+SPI0_CH0CTRL_def, SPI0_PA_RANGE_def, SPI0_END_def, SPI0_START_def,
+SPI0_SYSCONFIG_def, SPI0_MODULCTRL_def, SPI0_CH0CONF_def] >>
+FULL_SIMP_TAC (std_ss++WORD_ss++WORD_BIT_EQ_ss) [] >>
+rw [local_tr_cases,driver_tr_cases,call_back_dr_state_def,call_back_dr_data_def,
+call_back_dr_def]  >>
+fs [ref_rel_def,IS_STATE_REL_def]]);  
+         
 val _ = export_theory();
